FormaleSystemeInLean/LectureAndExercise/FintypeSetDecidableEq.lean
@@ -1,0 +1,77 @@
+import FormaleSystemeInLean.LectureAndExercise.Powertype
+
+-- to do: warum brauchen wir diese instanz -> kurzen text dazu verfassen
+--
+
+theorem toSet_eq_iff_lists_have_same_members (X Y : Set α) (l k : List α) : l.toSet = X → k.toSet = Y → ((∀ a, a ∈ l ↔ a ∈ k) ↔ X = Y) := by
+  intro X_eq Y_eq
+  unfold List.toSet at *
+  constructor
+  . intro mem_iff
+    apply Set.ext
+    intro x
+    constructor
+    . intro x_mem
+      rw [← X_eq] at x_mem
+      rw [← Y_eq]
+      simp only [Membership.mem] at *
+      specialize mem_iff x
+      apply mem_iff.mp x_mem
+    . intro x_mem
+      rw [← Y_eq] at x_mem
+      rw [← X_eq]
+      simp only [Membership.mem] at *
+      specialize mem_iff x
+      apply mem_iff.mpr x_mem
+  . intro xy_eq
+    intro x
+    rw [← X_eq, ← Y_eq] at xy_eq
+    grind
+
+theorem set_eq_iff_filter_has_same_members (α : Type u) (h : ∀ (S : Set α), DecidablePred S) (T : Fintype α) (X Y : Set α) : X = Y ↔ (∀ a, a ∈ T.elems.filter ( · ∈ X) ↔ a ∈ T.elems.filter ( · ∈ Y)) := by
+  constructor
+  . intro xy_eq
+    intro x
+    simp only [List.mem_filter, decide_eq_true_eq, and_congr_right_iff]
+    intro x_mem
+    rw [xy_eq]
+  . intro h
+    simp only [List.mem_filter, decide_eq_true_eq, and_congr_right_iff] at h
+    apply Set.ext
+    intro x
+    have x_mem_elems := T.complete x
+    apply h x x_mem_elems
+
+theorem set_eq_iff_filter_eq (α : Type u) (h : ∀ (S : Set α), DecidablePred S) (T : Fintype α) (X Y : Set α) : X = Y ↔ T.elems.filter ( · ∈ X) = T.elems.filter ( · ∈ Y) := by
+  constructor
+  . intro eq
+    rw [eq]
+  . intro eq
+    apply Set.ext
+    intro x
+    constructor
+    . intro x_mem
+      have x_mem_filter : x ∈ T.elems.filter ( · ∈ X ) := by
+        simp only [List.mem_filter, decide_eq_true_eq]
+        constructor
+        . apply T.complete x
+        . exact x_mem
+      rw [eq] at x_mem_filter
+      grind
+    . intro x_mem
+      have x_mem_filter : x ∈ T.elems.filter ( · ∈ Y ) := by
+        simp only [List.mem_filter, decide_eq_true_eq]
+        constructor
+        . apply T.complete x
+        . exact x_mem
+      rw [← eq] at x_mem_filter
+      grind
+
+instance {α : Type u} [T : Fintype α] [DecidableEq α] [h : ∀ (S : Set α), DecidablePred S] : DecidableEq (Set α) := by
+  intro X Y
+  have aux := set_eq_iff_filter_eq α h T X Y
+  simp only [aux]
+  by_cases h : List.filter (fun x => decide (x ∈ X)) Fintype.elems
+    = List.filter (fun x => decide (x ∈ Y)) Fintype.elems
+  . apply isTrue h
+  . apply isFalse h
