FormaleSystemeInLean/LectureAndExercise/List.lean
@@ -1,0 +1,41 @@
+
+theorem List.removeAll_nil_flatten [BEq α] : ∀ (l : List (List α)), (l.removeAll [[]]).flatten = l.flatten := by
+  intro l
+  induction l with
+  | nil =>
+    simp
+  | cons a l ih =>
+    rw [List.cons_removeAll]
+    by_cases h : [[]].contains a
+    . have a_eq : a=[] := by simp_all
+      simp only [h]
+      rw [a_eq, List.flatten_cons, List.nil_append, if_neg]
+      . exact ih
+      . trivial
+    . simp only [h]
+      rw [if_true]
+      have a_eq : ¬(a = []) := by simp_all
+      rw [List.flatten_cons, ih]
+      rfl
+
+def List.removeDups [DecidableEq α] : List α -> List α
+  | [] => []
+  | hd::tl => if hd ∈ tl then tl.removeDups else hd::(tl.removeDups)
+
+theorem List.mem_removeDups [DecidableEq α] (l : List α) : ∀ a, a ∈ l ↔ a ∈ l.removeDups := by
+  induction l with
+  | nil =>
+    intro a
+    simp only [removeDups]
+  | cons b l' ih =>
+    unfold removeDups
+    intro a
+    by_cases b_mem : b ∈ l'
+    . simp only [b_mem, ite_true, List.mem_cons, ih]
+      by_cases a_eq : a = b
+      . simp only [a_eq, true_or]
+        specialize ih b
+        have aux : b ∈ l'.removeDups := ih.mp b_mem
+        simpa using aux
+      . simp only [a_eq, false_or]
+    . simp only [b_mem, ite_false, List.mem_cons, ih]
